

Question 6, Homework 1, Katie Hutchinson, che9vz

$$(1) m(a+bX) = a + b \times m(X)$$

$$\begin{aligned} m(a+bX) &= \frac{1}{N} \sum_{i=1}^N a + bX_i \\ &= \frac{1}{N} \left(\sum_{i=1}^N a + \sum_{i=1}^N bX_i \right) \\ &\quad \uparrow a \text{ is a constant} \\ &= \frac{1}{N} \left(Na + b \sum_{i=1}^N X_i \right) \\ &\quad \uparrow b \text{ is a constant} \\ &= a + b \left(\frac{1}{N} \sum_{i=1}^N X_i \right) \\ &\quad \uparrow m(X) \\ m(a+bX) &= a + b \times m(X) \end{aligned}$$

$$\begin{aligned} (2) \operatorname{cov}(X, X) &= s^2 \\ &= \frac{1}{N} \sum_{i=1}^N (X_i - m(X))(X_i - m(X)) \\ &= \frac{1}{N} \sum_{i=1}^N (X_i - m(X))^2 \\ &= s^2 \leftarrow \text{by definition} \end{aligned}$$

$$\begin{aligned} (3) \operatorname{cov}(X, a+bY) &= b \times \operatorname{cov}(X, Y) \\ &= \frac{1}{N} \sum_{i=1}^N (X_i - m(X))(a + bY_i - m(a + bY)) \\ &\quad \rightarrow Z_i = a + bY_i \\ &= \frac{1}{N} \sum_{i=1}^N (X_i - m(X))(Z_i - m(a + bY)) \\ &\quad \rightarrow m(a + bY) = a + b m(Y) \\ &= \frac{1}{N} \sum_{i=1}^N (X_i - m(X)) \underbrace{((a + bY_i) - (a + b m(Y)))}_{(a + bY_i - a - b m(Y))} \\ &\quad (bY_i - b m(Y)) \\ &\quad (b(Y_i - m(Y))) \end{aligned}$$

$$\frac{1}{N} \sum_{i=1}^N (X_i - m(X))(b(Y_i - m(Y)))$$

$$b \times \frac{1}{N} \sum_{i=1}^N (X_i - m(X))(Y_i - m(Y))$$

$$= b \times \operatorname{cov}(X, Y)$$

$$\begin{aligned} (4) \operatorname{cov}(a+bX, a+bY) &= b^2 \operatorname{cov}(X, Y) \\ &= \frac{1}{N} \sum_{i=1}^N (a + bX_i - m(a + bX))(a + bY_i - m(a + bY)) \\ &\quad (a + bX_i - m(a + bX)) \\ &\quad (a + bX_i - a - b(mX)) \\ &\quad (a + bX_i - a - b mX) \\ &\quad (bX_i - b(mX)) \\ &\quad [b(X_i - m(X))][b(Y_i - m(Y))] \\ &= \frac{b^2}{N} \sum_{i=1}^N (X_i - mX)(Y_i - mY) \\ &= b^2 \operatorname{cov}(X, Y) \end{aligned}$$

$$(5) \operatorname{med}(a+bX) = a + b \times \operatorname{med}(X)$$

Yes, the median only depends on the order of the data. Adding or simply shifts all the points by the same amount, while multiplying it by b stretches out the points. In both transformations, the order is still the same.

$$\operatorname{IQR}(a+bX) = a + b \times \operatorname{IQR}(X)$$

$$Q1(a+bX) = a + bQ1(X)$$

$$Q3(a+bX) = a + bQ3(X)$$

↓

$$\begin{aligned} \operatorname{IQR}(a+bX) &= (a + bQ3) - (a + bQ1) \\ &= b(Q3 - Q1) \\ &= b \operatorname{IQR}(X) \end{aligned}$$

This is not true since $\operatorname{IQR}(a+bX)$ is equal to $b \operatorname{IQR}(X)$ instead of $a + b \operatorname{IQR}(X)$.

$$\begin{aligned} (6) \text{ Ex: } X &= \xi 1, 43 \quad \left. \begin{array}{l} X^2 = \xi 1, 163 \\ m(X) = \frac{1+4}{2} = 2.5 \\ (m(X))^2 = 6.25 \end{array} \right\} \begin{array}{l} m(X^2) = \frac{1+16}{2} = 8.5 \\ 8.5 \neq 6.25 \end{array} \end{aligned}$$

$$\sqrt{X} = \xi 1, 2$$

$$m(\sqrt{X}) = \frac{1+2}{2} = 1.5$$

$$\sqrt{m(X)} = \sqrt{6.25} = 2.5$$

$$1.5 \neq 1.58$$